extraction.v
@@ -3,10 +3,10 @@ Require Import "sequentialconsistency".
 Extraction Language Haskell.
 Extract Constant current => "()".
 Extract Constant kE => "\x->x".
-Extract Constant agent => "Agent".
+Extract Constant agent => "AgentType".
 Extract Constant knowledge "d" => "NVar d".
 Extract Constant U => "()".
-Extract Constant IO "a" => "IO a".
+Extract Constant io "a" => "Prelude.IO a".
 
 Recursive Extraction motto_comm.
 
